WIP: Define overapproximation for RPC

ExistentialRules/ChaseSequence/Nontermination/Unblockability.lean
@@ -19,14 +19,133 @@ public section
 
 variable {sig : Signature} [DecidableEq sig.P] [DecidableEq sig.C] [DecidableEq sig.V]
 
+-- TODO: This is close to ObsolescenceCondition.propagates_under_constant_mapping; maybe we can unify this but maybe not, I think now this is sufficiently different
+
+@[expose]
+def ObsolescenceCondition.propagates_under_term_mapping_of_no_fresh_term_occurs (obs : ObsolescenceCondition sig) : Prop := ∀ {trg : PreTrigger sig} {fs : FactSet sig} {h : GroundTermMapping sig}, (∀ i lt t, t ∈ trg.fresh_terms_for_head_disjunct i lt -> t ∉ fs.terms) -> (∀ c ∈ trg.rule.head_constants, h (.const c) = .const c) -> obs.cond trg fs -> obs.cond { rule := trg.rule, subs := h ∘ trg.subs } (h.applyFactSet fs)
+
+theorem SkolemObsolescence.propagates_under_term_mapping_of_no_fresh_term_occurs :
+    (SkolemObsolescence sig).propagates_under_term_mapping_of_no_fresh_term_occurs := by
+  intro trg fs h no_fresh_term_occurs id_const cond
+  simp only [SkolemObsolescence] at cond
+  simp only [SkolemObsolescence]
+  rcases cond with ⟨i, lt, cond⟩
+  exists i, lt
+  intro f f_mem
+  suffices f ∈ h.applyFactSet (trg.mapped_head[i]'(by grind)).toSet by
+    apply TermMapping.apply_generalized_atom_set_subset_of_subset
+    . exact cond
+    . exact this
+  rw [List.mem_toSet] at f_mem
+  unfold PreTrigger.mapped_head at f_mem
+  simp only [List.getElem_map, List.getElem_attach, List.getElem_zipIdx, List.mem_map, Nat.zero_add] at f_mem
+  rcases f_mem with ⟨a, a_mem, f_eq⟩
+  rw [TermMapping.mem_apply_generalized_atom_set]
+  exists trg.apply_to_function_free_atom i lt a; constructor
+  . rw [List.mem_toSet]; simp only [PreTrigger.mapped_head, List.getElem_map, List.getElem_attach, List.getElem_zipIdx, Nat.zero_add, List.mem_map]; exists a
+  . rw [← f_eq, GeneralizedAtom.mk.injEq]
+    simp only [PreTrigger.apply_to_function_free_atom, TermMapping.apply_generalized_atom, true_and]
+    rw [List.map_map, List.map_inj_left]
+    intro voc voc_mem; rw [Function.comp_apply]
+    cases voc with
+    | const c =>
+      rw [PreTrigger.apply_to_var_or_const_for_const]
+      rw [PreTrigger.apply_to_var_or_const_for_const]
+      apply Eq.symm; apply id_const
+      simp only [Rule.head_constants, List.mem_flatMap]; exists trg.rule.head[i]; constructor; exact List.getElem_mem _
+      rw [FunctionFreeConjunction.mem_consts]; exists a
+    | var v =>
+      suffices v ∉ trg.rule.existential_vars_for_head_disjunct i lt by
+        rw [PreTrigger.apply_to_var_or_const_of_not_mem_existential_vars trg _ _ _ this]
+        rw [PreTrigger.apply_to_var_or_const_of_not_mem_existential_vars {rule := trg.rule, subs := h ∘ trg.subs} _ _ _ this]
+        simp
+      intro contra; apply no_fresh_term_occurs i lt (trg.functional_term_for_var i lt v contra)
+      . apply trg.mem_fresh_terms_of_functional_for_exis_var
+      . exists trg.apply_to_function_free_atom i lt a; constructor
+        . apply cond; rw [List.mem_toSet]; simp only [PreTrigger.mapped_head, List.getElem_map, List.getElem_attach, List.getElem_zipIdx, Nat.zero_add, List.mem_map]; exists a
+        . simp only [PreTrigger.apply_to_function_free_atom, TermMapping.apply_generalized_atom]
+          rw [List.mem_map]; exists .var v; constructor; exact voc_mem
+          rw [trg.apply_to_var_or_const_of_mem_existential_vars _ _ _ contra]
+
+theorem RestrictedObsolescence.propagates_under_term_mapping_of_no_fresh_term_occurs :
+    (RestrictedObsolescence sig).propagates_under_term_mapping_of_no_fresh_term_occurs := by
+  intro trg fs h _ id_const cond -- no_fresh_term_occurs is only needed for SkolemObsolescence
+  simp only [RestrictedObsolescence, PreTrigger.satisfied, PreTrigger.satisfied_for_disj] at cond
+  simp only [RestrictedObsolescence, PreTrigger.satisfied, PreTrigger.satisfied_for_disj]
+  rcases cond with ⟨i, lt, cond⟩
+  exists i, lt
+  rcases cond with ⟨s, id_front, cond⟩
+  exists h ∘ s;
+  constructor
+  . intro v v_mem; simp only [Function.comp_apply]; rw [id_front v v_mem]
+  . rw [GroundSubstitution.apply_function_free_conj_compose]
+    . rw [← TermMapping.apply_generalized_atom_set_toSet]
+      apply TermMapping.apply_generalized_atom_set_subset_of_subset
+      exact cond
+    . intro d d_mem; apply id_const
+      simp only [Rule.head_constants, List.mem_flatMap]; exists trg.rule.head[i]; constructor; exact List.getElem_mem _; exact d_mem
+
+variable {obs : ObsolescenceCondition sig}
+
 /-- A trigger is unblockable for a given `HeadChoice` if, for every derivation, when the trigger is loaded in a node of the branch indicated by the `HeacChoice`, then the `HeadChoice` result of the trigger also occurs in that branch. In the introducing paper this is called g-unblockable. -/
 @[expose]
 def Trigger.unblockable
-    {obs : ObsolescenceCondition sig}
-    (trg : Trigger obs.toLaxObsolescenceCondition)
     (rules : RuleSet sig)
-    (hc : HeadChoice sig) : Prop :=
-  ∀ td : RegularTreeDerivation obs rules, ∀ node : (td.subderivation_for_headChoice hc).Node, trg.loaded node.val.facts ->
-  ∃ node2 : (td.subderivation_for_headChoice hc).Node, node ≼ node2 ∧
+    (hc : HeadChoice sig)
+    (trg : Trigger obs.toLaxObsolescenceCondition) : Prop :=
+  ∀ kb : KnowledgeBase sig, kb.rules = rules ->
+  ∀ ct : RegularChaseTree obs kb, ∀ node : (ct.subderivation_for_headChoice hc).Node, trg.loaded node.val.facts ->
+  ∃ node2 : (ct.subderivation_for_headChoice hc).Node, node ≼ node2 ∧
   (trg.output_for_headChoice hc).toSet ⊆ node2.val.facts
+
+/-- This is Definition 7 from the [RPC] paper. -/
+def FactSet.is_rpc_overapproximation
+    (rules : RuleSet sig)
+    (hc : HeadChoice sig)
+    (trg : Trigger obs.toLaxObsolescenceCondition)
+    (fs : FactSet sig) : Prop :=
+  ∃ h : GroundTermMapping sig, (∀ t ∈ trg.mapped_frontier, h t = t) ∧
+    ∀ kb : KnowledgeBase sig, kb.rules = rules ->
+    ∀ ct : RegularChaseTree obs kb, ∀ node ∈ (ct.subderivation_for_headChoice hc).toChaseDerivation,
+      (¬ (trg.output_for_headChoice hc).toSet ⊆ node.facts) -> h.applyFactSet node.facts ⊆ fs
+
+/-- This is Lemma 1 from the [RPC] paper. -/
+theorem PreTrigger.unblockable_of_not_obsolete_for_overapproximation
+    (obs_propagates : obs.propagates_under_term_mapping_of_no_fresh_term_occurs)
+    {rules : RuleSet sig} {hc : HeadChoice sig} {trg : RTrigger obs rules} {fs : FactSet sig} :
+    fs.is_rpc_overapproximation rules hc trg.val -> ¬ obs.cond trg.val fs -> trg.val.unblockable rules hc := by
+  intro ⟨h, id_frontier, overapprox⟩ not_obs
+  intro kb rules_eq ct node loaded
+  let trg_kb : RTrigger obs kb.rules := ⟨trg.val, by rw [rules_eq]; exact trg.property⟩
+  suffices ∃ node2, node ≼ node2 ∧ ¬ trg.val.active node2.val.facts by
+    rcases this with ⟨node2, prec, not_active⟩
+    exists node2; constructor; exact prec
+    apply Classical.byContradiction
+    intro contra
+    apply not_active; constructor; exact Set.subset_trans loaded (RegularChaseDerivationSkeleton.facts_node_subset_of_prec prec)
+    intro is_obs; apply not_obs
+    suffices obs.cond trg.val (h.applyFactSet node2.val.facts) by
+      apply LaxObsolescenceCondition.monotone _ _ this
+      apply overapprox _ rules_eq _ _ node2.property
+      exact contra
+    apply (obs.preserved_under_equiv _).mp (obs_propagates _ _ is_obs)
+    . apply PreTrigger.equiv_of_rule_eq_of_mapped_frontier_equiv; rfl
+      rw [← PreTrigger.apply_mapping_after_mapped_frontier]
+      apply List.map_id_of_id_on_all_mem; exact id_frontier
+    . intro i lt t t_fresh t_mem_node2; apply contra
+      rcases RegularChaseBranch.trigger_introducing_functional_term_occurs_in_chase node2 t_mem_node2 (trg := trg_kb) t_fresh with ⟨node3, node3_prec, orig, orig_mem, equiv, headIdx_eq⟩
+      apply Set.subset_trans _ (RegularChaseDerivationSkeleton.facts_node_subset_of_prec node3_prec)
+      -- oh, I think the rest only holds if the headChoice is consistent for equivalent triggers (which we do not enforce at the moment)...
+      suffices trg.val.output_for_headChoice hc = orig.fst.val.output_for_headChoice hc by
+        rw [this]; simp only [PreTrigger.output_for_headChoice]
+        suffices RegularChaseNode.regularChaseNodeInstance.adheres_to_headChoice node3.val hc by
+          simp only [← this orig orig_mem]
+          exact node3.val.facts_contain_origin_result orig orig_mem
+        sorry
+      sorry
+    . sorry -- I think be just need to add this as another condition to `is_rpc_overapproximation`; in the original paper constants were simply not allowed in rules
+  rcases RegularChaseDerivation.fairness_prec (cd := (ct.subderivation_for_headChoice hc).toChaseDerivation) trg_kb with ⟨fairness_node, fair⟩
+  cases ChaseDerivationSkeleton.predecessor_total node fairness_node with
+  | inl prec => exists fairness_node; constructor; exact prec; apply fair; grind
+  | inr prec => exists node; constructor; grind; apply fair; exact prec
 
